<?xml version="1.0"?>

<!DOCTYPE rdf:RDF [
    <!ENTITY ldreg "http://ldreg.org/terms#" >
    <!ENTITY owl "http://www.w3.org/2002/07/owl#" >
    <!ENTITY xsd "http://www.w3.org/2001/XMLSchema#" >
    <!ENTITY rdfs "http://www.w3.org/2000/01/rdf-schema#" >
    <!ENTITY rdf "http://www.w3.org/1999/02/22-rdf-syntax-ns#" >
    <!ENTITY dc 'http://purl.org/dc/elements/1.1/'>
]>


<rdf:RDF 
    xmlns="http://ldreg.org/terms#"
    xml:base="http://ldreg.org/terms#"
    xmlns:ldreg="http://ldreg.org/terms#"
    xmlns:rdfs="http://www.w3.org/2000/01/rdf-schema#"
    xmlns:owl2xml="http://www.w3.org/2006/12/owl2-xml#"
    xmlns:owl="http://www.w3.org/2002/07/owl#"
    xmlns:xsd="http://www.w3.org/2001/XMLSchema#"
    xmlns:rdf="http://www.w3.org/1999/02/22-rdf-syntax-ns#"
    xmlns:dc="&dc;"
>

  <owl:Ontology rdf:about="">
    <dc:creator rdf:resource="http://www.w3.org/People/Sandro/data#Sandro_Hawke"/>
    <rdfs:seeAlso rdf:resource="http://ldreg.net/wiki/Terminology"/>
  </owl:Ontology>
    
  <owl:ObjectProperty rdf:about="tracker">
    <rdfs:comment>Which tracker(s) are used for tracking usage of this vocabulary?</rdfs:comment>
    <rdfs:range rdf:resource="Tracker"/>
    <rdfs:domain rdf:resource="VocabularySource"/>
  </owl:ObjectProperty>
    
  <owl:Class rdf:about="DataSource">
    <rdfs:comment>An RDF graph available on the Web.</rdfs:comment>
  </owl:Class>
  
  <owl:Class rdf:about="Tracker">
    <rdfs:comment>A tracker is a database (with a standard Web API) operating on behalf of the owners of one or more vocabularies, maintaining a list of the data sources which use each term in the vocabulary.</rdfs:comment>
  </owl:Class>
    
  <owl:Class rdf:about="VocabularySource">
    <rdfs:comment>A vocabulary source is a data source which is also a vocabulary graph. This is, it is a data source which has an identity IRI which is the namespace part of one or more terms.</rdfs:comment>
    <rdfs:subClassOf rdf:resource="DataSource"/>
  </owl:Class>
    
  <rdf:Description rdf:about="http://ldreg.org/terms#">
    <tracker rdf:resource="http://ldreg.rdftracker.com"/>
  </rdf:Description>
    
  <Tracker rdf:about="http://ldreg.rdftracker.com"/>

</rdf:RDF>

